

Warning: in propositional logic, we had a failsafe procedure for determining whether an argument was valid or invalid. We don't have such a failsafe procedure for quantificational logic. So figuring out which arguments are valid and which aren't requires *a bunch of practice*.

Here's a reminder of the new rules:

$$\begin{array}{l|l} l & \forall v\varphi \\ m & \varphi(\tau/v) \quad \forall E, l \end{array}$$

$$\begin{array}{l|l} l & \varphi(\tau/v) \\ m & \exists v\varphi \quad \exists I, l \end{array}$$

$$\begin{array}{l|l} l & \varphi(\tau/v) \\ m & \forall v\varphi \quad \forall I, l \end{array}$$

provided τ does not occur in φ or in any undischarged assumption.

$$\begin{array}{l|l} k & \exists v\varphi \\ l & \varphi(a/x) \rightarrow \psi \\ n & \psi \quad \text{E}\exists k, l \end{array}$$

where a occurs neither in ψ nor in $\exists v\varphi$ nor in an undischarged assumption.

1. Build a model to show the following argument is invalid: $\forall x(Px \rightarrow Qx), Qa \vdash Pa$.

Domain: 0

P_- :

Q_- : 0

a : 0

2. Try (and fail!) to build a model to show the following argument is invalid: $\forall x(Px \rightarrow Qx), Pa \vdash Qa$. Then, prove the argument.

Proof:

| | | |
|---|--------------------------------|---------------------|
| 1 | $\forall x(Px \rightarrow Qx)$ | Assumption |
| 2 | Pa | Assumption |
| 3 | $Pa \rightarrow Qa$ | E \forall 1 |
| 4 | Qa | E \rightarrow 2,3 |

3. What is the mistake in the following proof?

| | | | |
|---|--|-----------------|--|
| 1 | | $\forall x Rxa$ | Assumption |
| 2 | | Rba | $E\forall$ 1 |
| 3 | | $\forall y Rby$ | $I\forall$ 2 You can't generalize about a , since it is not an undischarged assumption |

4. What is the mistake in the following proof?

| | | | |
|---|--|---------------------------------|---|
| 1 | | $\forall x (Px \rightarrow Qx)$ | Assumption |
| 2 | | $Pa \rightarrow Qb$ | $E\forall$ 1 When you eliminate a \forall , you must replace the variable with the <i>same</i> constant |

5. What is the mistake in the following proof?

| | | | |
|---|--|-----------------|------------|
| 1 | | $\exists x Qxb$ | Assumption |
| 2 | | | |
| 3 | | | |
| 4 | | | |
| 5 | | | |

| | | | |
|---|--|---------------------------------|--------------------|
| 2 | | Qbb | Assumption |
| 3 | | $\exists x Qxx$ | $I\exists$ 2 |
| 4 | | $Qbb \rightarrow \exists x Qxx$ | $I\rightarrow$ 2-3 |
| 5 | | $\exists x Qxx$ | $E\exists$ 1,4 |

The antecedent of the conditional that is used to eliminate \exists must have the 'x' replaced with a constant that doesn't appear in the proof.

6. Prove the following arguments:

(a) $\forall xPx, \forall x(Px \rightarrow Qx) \vdash \forall xQx$

| | | |
|---|--------------------------------|--------------------|
| 1 | $\forall xPx$ | Assumption |
| 2 | $\forall x(Px \rightarrow Qx)$ | Assumption |
| 3 | Pa | $E\forall$ 1 |
| 4 | $Pa \rightarrow Qa$ | $E\forall$ 2 |
| 5 | Qa | $E\rightarrow$ 3,4 |
| 6 | $\forall xQx$ | $I\forall$ 5 |

(b) $\vdash \forall xRax \rightarrow (\exists y\forall xRyx \wedge Rab)$

| | | |
|---|------------------------------------|--------------|
| 1 | $\forall xRax$ | Assumption |
| 2 | $\exists y\forall xRyx$ | $I\exists$ 1 |
| 3 | Rab | $E\forall$ 1 |
| 4 | $\exists y\forall xRyx \wedge Rab$ | $I\wedge$ 1 |

(c) $\forall xPx \vee \forall xQx \vdash \forall y(Py \vee (Qy \vee Ry))$

| | | |
|----|---|---------------------|
| 1 | $\forall xPx \vee \forall xQx$ | Assumption |
| 2 | $\forall xPx$ | Assumption |
| 3 | Pa | $E\forall$ 2 |
| 4 | $Pa \vee (Qa \vee Ra)$ | $I\vee$ 3 |
| 5 | $\forall y(Py \vee (Qy \vee Ry))$ | $I\forall$ 4 |
| 6 | $\forall xPx \rightarrow \forall y(Py \vee (Qy \vee Ry))$ | $I\rightarrow$ 2-5 |
| 7 | $\forall xQx$ | Assumption |
| 8 | Qa | $E\forall$ 7 |
| 9 | $Qa \vee Ra$ | $I\vee$ 8 |
| 10 | $Pa \vee (Qa \vee Ra)$ | $I\vee$ 9 |
| 11 | $\forall y(Py \vee (Qy \vee Ry))$ | $I\forall$ 10 |
| 12 | $\forall xQx \rightarrow \forall y(Py \vee (Qy \vee Ry))$ | $I\rightarrow$ 7-11 |
| 13 | $\forall y(Py \vee (Qy \vee Ry))$ | $E\vee$ 1,6, 12 |

(d) $\forall x(Px \rightarrow (Qx \wedge Rx)), \exists xPx \vdash \exists xRx$

| | | |
|---|--|---------------------|
| 1 | $\forall x(Px \rightarrow (Qx \wedge Rx))$ | Assumption |
| 2 | $\exists xPx$ | Assumption |
| 3 | Pa | Assumption |
| 4 | $Pa \rightarrow (Qa \wedge Ra)$ | E \forall 1 |
| 5 | $Qa \wedge Ra$ | E \rightarrow 3,4 |
| 6 | Ra | E \wedge 5 |
| 7 | $\exists xRx$ | I \exists 6 |
| 8 | $Pa \rightarrow \exists xRx$ | I \rightarrow 3-7 |
| 9 | $\exists xRx$ | E \exists 2,8 |

(e) Hardest proof (and only doable after Wednesday): $\vdash \exists x(Fx \rightarrow \forall yFy)$ **Email me!**